WIP: Ddbec branch key id supplier (#72)

DynamoDbEncryption/runtimes/java/src/main/smithy-generated/software/amazon/cryptography/dynamoDbEncryption/DynamoDbItemBranchKeyIdSupplier.java
@@ -1,0 +1,83 @@
+// Copyright Amazon.com Inc. or its affiliates. All Rights Reserved.
+// SPDX-License-Identifier: Apache-2.0
+// Do not modify this file. This file is machine generated, and any changes to it will be overwritten.
+package software.amazon.cryptography.dynamoDbEncryption;
+
+import Dafny.Aws.Cryptography.DynamoDbEncryption.Types.Error;
+import Wrappers_Compile.Result;
+import java.lang.Exception;
+import java.lang.IllegalArgumentException;
+import java.util.Objects;
+import software.amazon.cryptography.dynamoDbEncryption.model.GetBranchKeyIdFromItemInput;
+import software.amazon.cryptography.dynamoDbEncryption.model.GetBranchKeyIdFromItemOutput;
+import software.amazon.cryptography.dynamoDbEncryption.model.NativeError;
+import software.amazon.cryptography.dynamoDbEncryption.model.OpaqueError;
+
+public final class DynamoDbItemBranchKeyIdSupplier implements IDynamoDbItemBranchKeyIdSupplier {
+  private final Dafny.Aws.Cryptography.DynamoDbEncryption.Types.IDynamoDbItemBranchKeyIdSupplier _impl;
+
+  private DynamoDbItemBranchKeyIdSupplier(
+      Dafny.Aws.Cryptography.DynamoDbEncryption.Types.IDynamoDbItemBranchKeyIdSupplier iDynamoDbItemBranchKeyIdSupplier) {
+    Objects.requireNonNull(iDynamoDbItemBranchKeyIdSupplier, "Missing value for required argument `iDynamoDbItemBranchKeyIdSupplier`");
+    this._impl = iDynamoDbItemBranchKeyIdSupplier;
+  }
+
+  public static DynamoDbItemBranchKeyIdSupplier wrap(
+      Dafny.Aws.Cryptography.DynamoDbEncryption.Types.IDynamoDbItemBranchKeyIdSupplier iDynamoDbItemBranchKeyIdSupplier) {
+    return new DynamoDbItemBranchKeyIdSupplier(iDynamoDbItemBranchKeyIdSupplier);
+  }
+
+  public static <I extends IDynamoDbItemBranchKeyIdSupplier> DynamoDbItemBranchKeyIdSupplier wrap(
+      I iDynamoDbItemBranchKeyIdSupplier) {
+    Objects.requireNonNull(iDynamoDbItemBranchKeyIdSupplier, "Missing value for required argument `iDynamoDbItemBranchKeyIdSupplier`");
+    if (iDynamoDbItemBranchKeyIdSupplier instanceof software.amazon.cryptography.dynamoDbEncryption.DynamoDbItemBranchKeyIdSupplier) {
+      return ((DynamoDbItemBranchKeyIdSupplier) iDynamoDbItemBranchKeyIdSupplier);
+    }
+    return DynamoDbItemBranchKeyIdSupplier.wrap(new NativeWrapper(iDynamoDbItemBranchKeyIdSupplier));
+  }
+
+  public Dafny.Aws.Cryptography.DynamoDbEncryption.Types.IDynamoDbItemBranchKeyIdSupplier impl() {
+    return this._impl;
+  }
+
+  public GetBranchKeyIdFromItemOutput GetBranchKeyIdFromItem(
+      GetBranchKeyIdFromItemInput nativeValue) {
+    Dafny.Aws.Cryptography.DynamoDbEncryption.Types.GetBranchKeyIdFromItemInput dafnyValue = ToDafny.GetBranchKeyIdFromItemInput(nativeValue);
+    Result<Dafny.Aws.Cryptography.DynamoDbEncryption.Types.GetBranchKeyIdFromItemOutput, Error> result = this._impl.GetBranchKeyIdFromItem(dafnyValue);
+    if (result.is_Failure()) {
+      throw ToNative.Error(result.dtor_error());
+    }
+    return ToNative.GetBranchKeyIdFromItemOutput(result.dtor_value());
+  }
+
+  private static final class NativeWrapper implements Dafny.Aws.Cryptography.DynamoDbEncryption.Types.IDynamoDbItemBranchKeyIdSupplier {
+    private final IDynamoDbItemBranchKeyIdSupplier _impl;
+
+    NativeWrapper(IDynamoDbItemBranchKeyIdSupplier nativeImpl) {
+      if (nativeImpl instanceof DynamoDbItemBranchKeyIdSupplier) {
+        throw new IllegalArgumentException("Recursive wrapping is strictly forbidden.");
+      }
+      this._impl = nativeImpl;
+    }
+
+    public Result<Dafny.Aws.Cryptography.DynamoDbEncryption.Types.GetBranchKeyIdFromItemOutput, Error> GetBranchKeyIdFromItem(
+        Dafny.Aws.Cryptography.DynamoDbEncryption.Types.GetBranchKeyIdFromItemInput dafnyInput) {
+      GetBranchKeyIdFromItemInput nativeInput = ToNative.GetBranchKeyIdFromItemInput(dafnyInput);
+      try {
+        GetBranchKeyIdFromItemOutput nativeOutput = this._impl.GetBranchKeyIdFromItem(nativeInput);
+        Dafny.Aws.Cryptography.DynamoDbEncryption.Types.GetBranchKeyIdFromItemOutput dafnyOutput = ToDafny.GetBranchKeyIdFromItemOutput(nativeOutput);
+        return Result.create_Success(dafnyOutput);
+      } catch (NativeError ex) {
+        return Result.create_Failure(ToDafny.Error(ex));
+      } catch (Exception ex) {
+        OpaqueError error = OpaqueError.builder().obj(ex).cause(ex).build();
+        return Result.create_Failure(ToDafny.Error(error));
+      }
+    }
+
+    public Result<Dafny.Aws.Cryptography.DynamoDbEncryption.Types.GetBranchKeyIdFromItemOutput, Error> GetBranchKeyIdFromItem_k(
+        Dafny.Aws.Cryptography.DynamoDbEncryption.Types.GetBranchKeyIdFromItemInput dafnyInput) {
+      throw NativeError.builder().message("Not supported at this time.").build();
+    }
+  }
+}
