DynamoDbEncryption/Model/AwsCryptographyDynamoDbEncryptionTypes.dfy
@@ -66,11 +66,17 @@ include "../../submodules/MaterialProviders/StandardLibrary/src/Index.dfy"
  predicate method IsValid_ConstructorPartList(x: seq<ConstructorPart>) {
  ( 1 <= |x|  )
 }
+ datatype CreateDynamoDbEncryptionBranchKeyIdSupplierInput = | CreateDynamoDbEncryptionBranchKeyIdSupplierInput (
+ nameonly ddbItemBranchKeyIdSupplier: IDynamoDbItemBranchKeyIdSupplier
+ )
+ datatype CreateDynamoDbEncryptionBranchKeyIdSupplierOutput = | CreateDynamoDbEncryptionBranchKeyIdSupplierOutput (
+ nameonly branchKeyIdSupplier: AwsCryptographyMaterialProvidersTypes.IBranchKeyIdSupplier
+ )
  class IDynamoDbEncryptionClientCallHistory {
  ghost constructor() {
- 
+ CreateDynamoDbEncryptionBranchKeyIdSupplier := [];
 }
- 
+ ghost var CreateDynamoDbEncryptionBranchKeyIdSupplier: seq<DafnyCallEvent<CreateDynamoDbEncryptionBranchKeyIdSupplierInput, Result<CreateDynamoDbEncryptionBranchKeyIdSupplierOutput, Error>>>
 }
  trait {:termination false} IDynamoDbEncryptionClient
  {
@@ -99,11 +105,99 @@ include "../../submodules/MaterialProviders/StandardLibrary/src/Index.dfy"
  predicate ValidState()
  ensures ValidState() ==> History in Modifies
   ghost const History: IDynamoDbEncryptionClientCallHistory
+ predicate CreateDynamoDbEncryptionBranchKeyIdSupplierEnsuresPublicly(input: CreateDynamoDbEncryptionBranchKeyIdSupplierInput , output: Result<CreateDynamoDbEncryptionBranchKeyIdSupplierOutput, Error>)
+ // The public method to be called by library consumers
+ method CreateDynamoDbEncryptionBranchKeyIdSupplier ( input: CreateDynamoDbEncryptionBranchKeyIdSupplierInput )
+ returns (output: Result<CreateDynamoDbEncryptionBranchKeyIdSupplierOutput, Error>)
+ requires
+ && ValidState()
+ && input.ddbItemBranchKeyIdSupplier.ValidState()
+ && input.ddbItemBranchKeyIdSupplier.Modifies !! {History}
+ modifies Modifies - {History} ,
+ input.ddbItemBranchKeyIdSupplier.Modifies ,
+ History`CreateDynamoDbEncryptionBranchKeyIdSupplier
+ // Dafny will skip type parameters when generating a default decreases clause.
+ decreases Modifies - {History} ,
+ input.ddbItemBranchKeyIdSupplier.Modifies
+ ensures
+ && ValidState()
+ && ( output.Success? ==> 
+ && output.value.branchKeyIdSupplier.ValidState()
+ && output.value.branchKeyIdSupplier.Modifies !! {History}
+ && fresh(output.value.branchKeyIdSupplier)
+ && fresh ( output.value.branchKeyIdSupplier.Modifies - Modifies - {History} - input.ddbItemBranchKeyIdSupplier.Modifies ) )
+ ensures CreateDynamoDbEncryptionBranchKeyIdSupplierEnsuresPublicly(input, output)
+ ensures History.CreateDynamoDbEncryptionBranchKeyIdSupplier == old(History.CreateDynamoDbEncryptionBranchKeyIdSupplier) + [DafnyCallEvent(input, output)]
  
 }
  datatype DynamoDbEncryptionConfig = | DynamoDbEncryptionConfig (
  
  )
+ class IDynamoDbItemBranchKeyIdSupplierCallHistory {
+ ghost constructor() {
+ GetBranchKeyIdFromItem := [];
+}
+ ghost var GetBranchKeyIdFromItem: seq<DafnyCallEvent<GetBranchKeyIdFromItemInput, Result<GetBranchKeyIdFromItemOutput, Error>>>
+}
+ trait {:termination false} IDynamoDbItemBranchKeyIdSupplier
+ {
+ // Helper to define any additional modifies/reads clauses.
+ // If your operations need to mutate state,
+ // add it in your constructor function:
+ // Modifies := {your, fields, here, History};
+ // If you do not need to mutate anything:
+// Modifies := {History};
+
+ ghost const Modifies: set<object>
+ // For an unassigned field defined in a trait,
+ // Dafny can only assign a value in the constructor.
+ // This means that for Dafny to reason about this value,
+ // it needs some way to know (an invariant),
+ // about the state of the object.
+ // This builds on the Valid/Repr paradigm
+ // To make this kind requires safe to add
+ // to methods called from unverified code,
+ // the predicate MUST NOT take any arguments.
+ // This means that the correctness of this requires
+ // MUST only be evaluated by the class itself.
+ // If you require any additional mutation,
+ // then you MUST ensure everything you need in ValidState.
+ // You MUST also ensure ValidState in your constructor.
+ predicate ValidState()
+ ensures ValidState() ==> History in Modifies
+  ghost const History: IDynamoDbItemBranchKeyIdSupplierCallHistory
+ predicate GetBranchKeyIdFromItemEnsuresPublicly(input: GetBranchKeyIdFromItemInput , output: Result<GetBranchKeyIdFromItemOutput, Error>)
+ // The public method to be called by library consumers
+ method GetBranchKeyIdFromItem ( input: GetBranchKeyIdFromItemInput )
+ returns (output: Result<GetBranchKeyIdFromItemOutput, Error>)
+ requires
+ && ValidState()
+ modifies Modifies - {History} ,
+ History`GetBranchKeyIdFromItem
+ // Dafny will skip type parameters when generating a default decreases clause.
+ decreases Modifies - {History}
+ ensures
+ && ValidState()
+ ensures GetBranchKeyIdFromItemEnsuresPublicly(input, output)
+ ensures History.GetBranchKeyIdFromItem == old(History.GetBranchKeyIdFromItem) + [DafnyCallEvent(input, output)]
+ {
+ output := GetBranchKeyIdFromItem' (input);
+ History.GetBranchKeyIdFromItem := History.GetBranchKeyIdFromItem + [DafnyCallEvent(input, output)];
+}
+ // The method to implement in the concrete class. 
+ method GetBranchKeyIdFromItem' ( input: GetBranchKeyIdFromItemInput )
+ returns (output: Result<GetBranchKeyIdFromItemOutput, Error>)
+ requires
+ && ValidState()
+ modifies Modifies - {History}
+ // Dafny will skip type parameters when generating a default decreases clause.
+ decreases Modifies - {History}
+ ensures
+ && ValidState()
+ ensures GetBranchKeyIdFromItemEnsuresPublicly(input, output)
+ ensures unchanged(History)
+ 
+}
  datatype DynamoDbTableEncryptionConfig = | DynamoDbTableEncryptionConfig (
  nameonly partitionKeyName: ComAmazonawsDynamodbTypes.KeySchemaAttributeName ,
  nameonly sortKeyName: Option<ComAmazonawsDynamodbTypes.KeySchemaAttributeName> ,
@@ -118,6 +212,12 @@ include "../../submodules/MaterialProviders/StandardLibrary/src/Index.dfy"
  type DynamoDbTableEncryptionConfigList = map<ComAmazonawsDynamodbTypes.TableName, DynamoDbTableEncryptionConfig>
  datatype DynamoDbTablesEncryptionConfig = | DynamoDbTablesEncryptionConfig (
  nameonly tableEncryptionConfigs: DynamoDbTableEncryptionConfigList
+ )
+ datatype GetBranchKeyIdFromItemInput = | GetBranchKeyIdFromItemInput (
+ nameonly ddbItem: ComAmazonawsDynamodbTypes.AttributeMap
+ )
+ datatype GetBranchKeyIdFromItemOutput = | GetBranchKeyIdFromItemOutput (
+ nameonly branchKeyId: string
  )
  datatype GetPrefix = | GetPrefix (
  nameonly length: int32
@@ -333,6 +433,34 @@ include "../../submodules/MaterialProviders/StandardLibrary/src/Index.dfy"
  && Operations.ValidInternalConfig?(config)
  && History !in Operations.ModifiesInternalConfig(config)
  && Modifies == Operations.ModifiesInternalConfig(config) + {History}
+ predicate CreateDynamoDbEncryptionBranchKeyIdSupplierEnsuresPublicly(input: CreateDynamoDbEncryptionBranchKeyIdSupplierInput , output: Result<CreateDynamoDbEncryptionBranchKeyIdSupplierOutput, Error>)
+ {Operations.CreateDynamoDbEncryptionBranchKeyIdSupplierEnsuresPublicly(input, output)}
+ // The public method to be called by library consumers
+ method CreateDynamoDbEncryptionBranchKeyIdSupplier ( input: CreateDynamoDbEncryptionBranchKeyIdSupplierInput )
+ returns (output: Result<CreateDynamoDbEncryptionBranchKeyIdSupplierOutput, Error>)
+ requires
+ && ValidState()
+ && input.ddbItemBranchKeyIdSupplier.ValidState()
+ && input.ddbItemBranchKeyIdSupplier.Modifies !! {History}
+ modifies Modifies - {History} ,
+ input.ddbItemBranchKeyIdSupplier.Modifies ,
+ History`CreateDynamoDbEncryptionBranchKeyIdSupplier
+ // Dafny will skip type parameters when generating a default decreases clause.
+ decreases Modifies - {History} ,
+ input.ddbItemBranchKeyIdSupplier.Modifies
+ ensures
+ && ValidState()
+ && ( output.Success? ==> 
+ && output.value.branchKeyIdSupplier.ValidState()
+ && output.value.branchKeyIdSupplier.Modifies !! {History}
+ && fresh(output.value.branchKeyIdSupplier)
+ && fresh ( output.value.branchKeyIdSupplier.Modifies - Modifies - {History} - input.ddbItemBranchKeyIdSupplier.Modifies ) )
+ ensures CreateDynamoDbEncryptionBranchKeyIdSupplierEnsuresPublicly(input, output)
+ ensures History.CreateDynamoDbEncryptionBranchKeyIdSupplier == old(History.CreateDynamoDbEncryptionBranchKeyIdSupplier) + [DafnyCallEvent(input, output)]
+ {
+ output := Operations.CreateDynamoDbEncryptionBranchKeyIdSupplier(config, input);
+ History.CreateDynamoDbEncryptionBranchKeyIdSupplier := History.CreateDynamoDbEncryptionBranchKeyIdSupplier + [DafnyCallEvent(input, output)];
+}
  
 }
 }
@@ -344,4 +472,25 @@ include "../../submodules/MaterialProviders/StandardLibrary/src/Index.dfy"
  type InternalConfig
  predicate ValidInternalConfig?(config: InternalConfig)
  function ModifiesInternalConfig(config: InternalConfig): set<object>
+ predicate CreateDynamoDbEncryptionBranchKeyIdSupplierEnsuresPublicly(input: CreateDynamoDbEncryptionBranchKeyIdSupplierInput , output: Result<CreateDynamoDbEncryptionBranchKeyIdSupplierOutput, Error>)
+ // The private method to be refined by the library developer
+
+
+ method CreateDynamoDbEncryptionBranchKeyIdSupplier ( config: InternalConfig , input: CreateDynamoDbEncryptionBranchKeyIdSupplierInput )
+ returns (output: Result<CreateDynamoDbEncryptionBranchKeyIdSupplierOutput, Error>)
+ requires
+ && ValidInternalConfig?(config)
+ && input.ddbItemBranchKeyIdSupplier.ValidState()
+ modifies ModifiesInternalConfig(config) ,
+ input.ddbItemBranchKeyIdSupplier.Modifies
+ // Dafny will skip type parameters when generating a default decreases clause.
+ decreases ModifiesInternalConfig(config) ,
+ input.ddbItemBranchKeyIdSupplier.Modifies
+ ensures
+ && ValidInternalConfig?(config)
+ && ( output.Success? ==> 
+ && output.value.branchKeyIdSupplier.ValidState()
+ && fresh(output.value.branchKeyIdSupplier)
+ && fresh ( output.value.branchKeyIdSupplier.Modifies - ModifiesInternalConfig(config) - input.ddbItemBranchKeyIdSupplier.Modifies ) )
+ ensures CreateDynamoDbEncryptionBranchKeyIdSupplierEnsuresPublicly(input, output)
 }
