DynamoDbEncryption/test/DynamoDbEncryption/DynamoDbEncryptionBranchKeyIdSupplierTest.dfy
@@ -1,0 +1,186 @@
+// Copyright Amazon.com Inc. or its affiliates. All Rights Reserved.
+// SPDX-License-Identifier: Apache-2.0
+include "../../../submodules/MaterialProviders/StandardLibrary/src/StandardLibrary.dfy"
+include "../../src/DynamoDbEncryption/Index.dfy"
+include "../../Model/AwsCryptographyDynamoDbEncryptionTypes.dfy"
+include "../../../submodules/MaterialProviders/ComAmazonawsDynamodb/Model/ComAmazonawsDynamodbTypes.dfy"
+include "../../../submodules/MaterialProviders/AwsCryptographicMaterialProviders/Model/AwsCryptographyMaterialProvidersTypes.dfy"
+include "../TestFixtures.dfy"
+
+module DynamoDbEncryptionBranchKeyIdSupplierTest {
+  import opened Wrappers
+  import opened StandardLibrary.UInt
+  import MaterialProviders
+  import DynamoDbEncryption
+  import Types = AwsCryptographyDynamoDbEncryptionTypes
+  import MPL = AwsCryptographyMaterialProvidersTypes
+  import KMS = Com.Amazonaws.Kms
+  import DDB = Com.Amazonaws.Dynamodb
+  import UTF8
+  import TestFixtures
+  import CSE = AwsCryptographyStructuredEncryptionTypes
+  import SE = StructuredEncryptionUtil
+  import Base64
+
+  const TEST_DBE_ALG_SUITE_ID := MPL.AlgorithmSuiteId.DBE(MPL.ALG_AES_256_GCM_HKDF_SHA512_COMMIT_KEY_SYMSIG_HMAC_SHA384);
+
+  // THIS IS A TESTING RESOURCE DO NOT USE IN A PRODUCTION ENVIRONMENT
+  const keyArn := "arn:aws:kms:us-west-2:370957321024:key/9d989aa2-2f9c-438c-a745-cc57d3ad0126";
+  const branchKeyStoreArn := "arn:aws:dynamodb:us-west-2:370957321024:table/HierarchicalKeyringTestTable";
+
+  // These tests require a keystore populated with a key with this Id
+  const BRANCH_KEY_ID := "hierarchy-test-v1";
+  const BRANCH_KEY_ID_UTF8 := UTF8.EncodeAscii("hierarchy-test-v1");
+  const ACTIVE_ACTIVE_BRANCH_KEY_ID := "hierarchy-test-active-active";
+
+  // Constants for TestBranchKeySupplier
+  const BRANCH_KEY := "branchKey";
+  const STRING_TYPE_ID: seq<uint8> := [0x00, 0x01];
+  const CASE_A := "CASE_A";
+  const CASE_B := "CASE_B";
+  // "CASE_A" encoded as a DDB S
+  const CASE_A_BYTES: seq<uint8> := STRING_TYPE_ID + [0x43, 0x41, 0x53, 0x45, 0x5f, 0x41];
+  // "CASE_B" encoded as a DDB S
+  const CASE_B_BYTES: seq<uint8> := STRING_TYPE_ID + [0x43, 0x41, 0x53, 0x45, 0x5f, 0x42];
+  const BRANCH_KEY_ID_A := BRANCH_KEY_ID
+  const BRANCH_KEY_ID_B := ACTIVE_ACTIVE_BRANCH_KEY_ID
+  const RESERVED_PREFIX := "aws-crypto-attr.";
+
+  method {:test} TestHappyCase() 
+  {
+    var ddbItemToBranchKeyId: Types.IDynamoDbItemBranchKeyIdSupplier := new TestBranchKeyIdSupplier();
+    var ddbEncResources :- expect DynamoDbEncryption.DynamoDbEncryption();
+    var branchKeyIdSupplierOut :- expect ddbEncResources.CreateDynamoDbEncryptionBranchKeyIdSupplier(
+      Types.CreateDynamoDbEncryptionBranchKeyIdSupplierInput(
+        ddbItemBranchKeyIdSupplier := ddbItemToBranchKeyId
+      )
+    );
+    var branchKeyIdSupplier := branchKeyIdSupplierOut.branchKeyIdSupplier;
+
+    var ttl : int64 := (1 * 60000) * 10;
+    var mpl :- expect MaterialProviders.MaterialProviders();
+    var kmsClient :- expect KMS.KMSClient();
+    var dynamodbClient :- expect DDB.DynamoDBClient();
+    var hierarchyKeyring :- expect mpl.CreateAwsKmsHierarchicalKeyring(
+      MPL.CreateAwsKmsHierarchicalKeyringInput(
+        branchKeyId := None,
+        branchKeyIdSupplier := Some(branchKeyIdSupplier),
+        kmsKeyId := keyArn,
+        kmsClient := kmsClient,
+        ddbClient := dynamodbClient,
+        branchKeyStoreArn := branchKeyStoreArn,
+        ttlSeconds := ttl,
+        maxCacheSize := Option.Some(10),
+        grantTokens := Option.None
+      )
+    );
+
+    var keyAttrName := UTF8.EncodeAscii(RESERVED_PREFIX + BRANCH_KEY);
+    
+    // Test Encryption Context with Case A
+    var materials :- expect mpl.InitializeEncryptionMaterials(
+      MPL.InitializeEncryptionMaterialsInput(
+        algorithmSuiteId := TEST_DBE_ALG_SUITE_ID,
+        encryptionContext := map[],
+        requiredEncryptionContextKeys := [],
+        signingKey := None,
+        verificationKey := None
+      )
+    );
+    var caseA :- expect UTF8.Encode(Base64.Encode(CASE_A_BYTES));
+    var contextCaseA := materials.encryptionContext[keyAttrName := caseA];
+    var materialsA := materials.(encryptionContext := contextCaseA);
+    TestRoundtrip(hierarchyKeyring, materialsA, TEST_DBE_ALG_SUITE_ID, BRANCH_KEY_ID_A); 
+
+    // Test Encryption Context with Case B
+    var caseB :- expect UTF8.Encode(Base64.Encode(CASE_B_BYTES));
+    var contextCaseB := materials.encryptionContext[keyAttrName := caseB];
+    var materialsB := materials.(encryptionContext := contextCaseB);
+    TestRoundtrip(hierarchyKeyring, materialsB, TEST_DBE_ALG_SUITE_ID, BRANCH_KEY_ID_B); 
+  }
+
+  method TestRoundtrip(
+    hierarchyKeyring: MPL.IKeyring,
+    encryptionMaterialsIn: MPL.EncryptionMaterials,
+    algorithmSuiteId: MPL.AlgorithmSuiteId,
+    expectedBranchKeyId: string
+  )
+    requires hierarchyKeyring.ValidState()
+    modifies hierarchyKeyring.Modifies
+    ensures hierarchyKeyring.ValidState()
+  {
+    var encryptionMaterialsOut :- expect hierarchyKeyring.OnEncrypt(
+      MPL.OnEncryptInput(materials:=encryptionMaterialsIn)
+    );
+    
+    var mpl :- expect MaterialProviders.MaterialProviders();
+    var _ :- expect mpl.EncryptionMaterialsHasPlaintextDataKey(encryptionMaterialsOut.materials);
+
+    expect |encryptionMaterialsOut.materials.encryptedDataKeys| == 1;
+
+    var edk := encryptionMaterialsOut.materials.encryptedDataKeys[0];
+    
+    // Verify the edk was created with the expected branch key
+    var expectedBranchKeyIdUTF8 :- expect UTF8.Encode(expectedBranchKeyId);
+    expect edk.keyProviderInfo == expectedBranchKeyIdUTF8;
+
+    var decryptionMaterialsIn :- expect mpl.InitializeDecryptionMaterials(
+      MPL.InitializeDecryptionMaterialsInput(
+        algorithmSuiteId := algorithmSuiteId,
+        encryptionContext := encryptionMaterialsIn.encryptionContext,
+        requiredEncryptionContextKeys := []
+      )
+    );
+    var decryptionMaterialsOut :- expect hierarchyKeyring.OnDecrypt(
+      MPL.OnDecryptInput(
+        materials:=decryptionMaterialsIn,
+        encryptedDataKeys:=[edk]
+      )
+    );
+
+    expect encryptionMaterialsOut.materials.plaintextDataKey
+    == decryptionMaterialsOut.materials.plaintextDataKey;
+  }
+
+  // returns "branchKeyIdA" when item contains "branchKey":"caseA"
+  // returns "branchKeyIdB" when item contains "branchKey":"caseB"
+  // otherwise returns a Failure
+  class TestBranchKeyIdSupplier extends Types.IDynamoDbItemBranchKeyIdSupplier
+  {
+    predicate ValidState()
+      ensures ValidState() ==> History in Modifies
+    {
+      History in Modifies
+    }
+
+    constructor()
+      ensures ValidState() && fresh(this) && fresh(History) && fresh(Modifies)
+    {
+      History := new Types.IDynamoDbItemBranchKeyIdSupplierCallHistory();
+      Modifies := {History};
+    }
+
+    predicate GetBranchKeyIdFromItemEnsuresPublicly(input: Types.GetBranchKeyIdFromItemInput, output: Result<Types.GetBranchKeyIdFromItemOutput, Types.Error>)
+    {true}
+
+    method GetBranchKeyIdFromItem'(input: Types.GetBranchKeyIdFromItemInput)
+        returns (output: Result<Types.GetBranchKeyIdFromItemOutput, Types.Error>)
+      requires ValidState()
+      modifies Modifies - {History}
+      decreases Modifies - {History}
+      ensures ValidState()
+      ensures GetBranchKeyIdFromItemEnsuresPublicly(input, output)
+      ensures unchanged(History)
+    {
+      var item := input.ddbItem;
+
+      if BRANCH_KEY in item.Keys && item[BRANCH_KEY].S? && item[BRANCH_KEY].S == CASE_A {
+        return Success(Types.GetBranchKeyIdFromItemOutput(branchKeyId:=BRANCH_KEY_ID_A));
+      } else if BRANCH_KEY in item.Keys && item[BRANCH_KEY].S? && item[BRANCH_KEY].S == CASE_B {
+        return Success(Types.GetBranchKeyIdFromItemOutput(branchKeyId:=BRANCH_KEY_ID_B));
+      } else {
+        return Failure(Types.DynamoDbEncryptionException(message := "Can't determine branchKeyId from item"));
+      }
+    }
+  }
+}
